Test/tutorial/ImpVerifiedCompiler/SemanticsProperties.dfy
@@ -49,6 +49,12 @@ lemma combine_reductions<T(!new)>()
 	star_trans<T>();
 }
 
+lemma plus_one<T(!new)>(R: (T,T) -> bool, conf1: T, conf2: T)
+	requires R(conf1,conf2)
+	ensures star(R,conf1,conf2)
+{
+}
+
 lemma plus_star<T(!new)>(R: (T,T) -> bool, conf1: T, conf2: T)
 	requires plus(R,conf1,conf2)
 	ensures star(R,conf1,conf2)
@@ -101,3 +107,76 @@ lemma infseq_if_all_seq_inf<T(!new)>(R: (T,T) -> bool, conf: T)
 {
 	infseq_if_all_seq_inf_pre(R,conf);
 }
+
+lemma infseq_coinduction_principle<T(!new)>(k: ORDINAL, R: (T,T) -> bool, X: T -> bool, a : T)
+	requires (forall a: T :: X(a) ==> exists b: T :: R(a,b) && X(b))
+	requires X(a)
+	ensures inf#[k](R,a)
+{
+	if k.Offset == 0 {} else {
+		var b :| R(a,b) && X(b);
+		infseq_coinduction_principle(k-1,R,X,b);
+	}
+}
+
+greatest lemma infseq_coinduction_principle_p<T(!new)>(R: (T,T) -> bool, X: T -> bool, a: T)
+	requires (forall a: T :: X(a) ==> exists b: T :: R(a,b) && X(b))
+	ensures  X(a) ==> inf(R,a)
+{
+	forall a: T ensures X(a) ==> inf(R,a) {
+		if X(a) {
+			var b :| R(a,b) && X(b);
+			infseq_coinduction_principle_p(R,X,a);
+		}
+	}
+}
+
+lemma infseq_coinduction_principle_p0<T(!new)>(R: (T,T) -> bool, X: T -> bool, a : T)
+	requires (forall a: T :: X(a) ==> exists b: T :: R(a,b) && X(b))
+	requires X(a)
+	ensures inf(R,a)
+{
+
+	if X(a) {
+		infseq_coinduction_principle_p(R,X,a);
+	}
+	
+}
+
+// lemma infseq_coinduction_principle_p2<T(!new)>(R: (T,T) -> bool, X: T -> bool)
+//	ensures (forall a: T :: X(a) ==> exists b: T :: R(a,b) && X(b)) ==> forall a: T :: X(a) ==> inf(R,a)
+// {
+// 	if (forall a: T :: X(a) ==> exists b: T :: R(a,b) && X(b)) {
+// 		infseq_coinduction_principle_p(R,X);
+// 	}
+// }
+
+lemma infseq_coinduction_principle_pre<T(!new)>(R: (T,T) -> bool, X: T -> bool,a: T)
+	requires (forall a: T :: X(a) ==> exists b: T :: plus(R,a, b) && X(b))
+	requires exists b: T :: star(R,a,b) && X(b)
+	ensures exists b: T :: R(a,b) && (exists c: T :: star(R,b,c) && X(c))
+{
+	var b: T :| star(R,a,b) && X(b);
+	if a == b {
+		var c :| plus(R,b, c) && X(c);
+	} else { 
+		var b0 :| R(a,b0) && star(R,b0,b);
+	}
+}
+
+lemma {:axiom} infseq_coinduction_principle_2<T(!new)>(R: (T,T) -> bool, X: T -> bool, a : T)
+	requires (forall a: T :: X(a) ==> exists b: T :: plus(R,a, b) && X(b))
+	requires X(a)
+	ensures inf(R,a)
+// {
+// 	assert exists b: T :: star(R,a,b) && X(b);
+// 	infseq_coinduction_principle_pre(R,X,a);
+	
+// 	//assume false;
+// 	// 	assume exists b: T :: star(R,a,b) && X(b);
+// // 	assume forall a: T :: (exists b: T :: star(R,a,b) && X(b)) ==> exists b: T :: R(a,b) && exists c: T :: star(R,b,c) && X(c);
+//  	//infseq_coinduction_principle_p0(R,(a: T) => exists b: T :: star(R,a,b) && X(b),a);
+//  	assume false;
+// }
+
+
