Test/tutorial/ImpVerifiedCompiler/SimulationRelationCont.dfy
@@ -3,6 +3,7 @@ include "ImpReductionContSem.dfy"
 include "Mach.dfy"
 include "MachSemantics.dfy"
 include "Compiler.dfy"
+include "SemanticsProperties.dfy"
 
 least predicate compile_cont(C: code, k: cont, pc: nat) {
 	if ! (pc < |C|) then false else
@@ -68,5 +69,40 @@ least lemma compile_cont_Kstop_inv(C: code, pc: nat, s: store)
 		case _ => 
 	}
 		
+}
+
+lemma compile_cont_Kseq_inv(C: code, c: com, k: cont, pc: nat, s: store)
+	requires compile_cont(C,(Kseq(c,k)),pc)
+	ensures exists pc': nat :: star((c1,c2) => transition(C,c1,c2),(pc, [], s),(pc', [], s)) && code_at(C,pc',compile_com(c)) && compile_cont(C,k,pc' + |compile_com(c)|)
+{
+}
+
+lemma compile_cont_Kwhile_inv(C: code, b: bexp, c: com, k: cont, pc: nat, s: store)
+	requires compile_cont(C,(Kwhile(b,c,k)),pc)
+	ensures exists pc': nat :: plus((c1,c2) => transition(C,c1,c2),(pc, [], s),(pc', [], s)) && code_at(C,pc',compile_com(c)) && compile_cont(C,k,pc' + |compile_com(CWhile(b,c))|)
+{
+
+	match C[pc] {
+
+		case Ibranch(ofs) => {
+
+			var pc': nat := pc + 1 + ofs;
+			var pc'': nat := pc' + |compile_com(CWhile(b, c))|;
+			assert pc' > 0;
+			assert pc'' > 0;	
+			assert code_at(C, pc', (compile_com(CWhile(b, c)))); 
+			assert compile_cont(C, k, pc'');
+
+			assert transition(C,(pc, [], s),(pc', [], s));
+			plus_one<configuration>((c1,c2) => transition(C,c1,c2),(pc, [], s),(pc', [], s));
+			
+			assume false;
+			
+		}
+
+		case _ => 
+		
+	}
+	
 }
 
